coq-osiris/theories/semantics/pure_wp.v
@@ -346,6 +346,8 @@ Inductive pure_wp {A E} : micro A E → (A → Prop) → (E → Prop) → Prop :
 
 Global Hint Constructors pure_wp : pure_wp.
 
+(* Definition disallowing exceptions *)
+Definition pure_wpv {A E} (m : micro A E) φ := pure_wp m φ (λ _, False).
 
 (** [pure_wp] is monotonic *)
 
@@ -500,11 +502,20 @@ Proof.
   intros e. rewrite discontinue_glue2. by constructor.
 Qed.
 
-Lemma pure_wp_try {A' A E E' φ ψ} m (f : A → micro A' E) (h : E' → micro A' E) :
+Lemma pure_wp_try {A' A E E' φ ψ} m (f : A → micro A' E') (h : E → micro A' E') :
   pure_wp m (λ a, pure_wp (f a) φ ψ) (λ e, pure_wp (h e) φ ψ) →
   pure_wp (try m f h) φ ψ.
 Proof.
   eauto using pure_wp_try2.
+Qed.
+
+Lemma pure_wp_orelse {A E} (m1 m2 : micro A E) φ ψ1 ψ :
+  pure_wp m1 φ ψ1 →
+  (∀ e, ψ1 e → pure_wp m2 φ ψ) →
+  pure_wp (orelse m1 m2) φ ψ.
+Proof.
+  intros. apply pure_wp_try2. eapply pure_wp_mono; eauto.
+  intro. rewrite continue_glue2. by constructor.
 Qed.
 
 Lemma pure_wp_bind_compat {A' A E} (φ : A → Prop) (ψ : E → Prop) (φ' : A' → Prop) m k :
@@ -514,6 +525,71 @@ Lemma pure_wp_bind_compat {A' A E} (φ : A → Prop) (ψ : E → Prop) (φ' : A'
 Proof.
   intros. eapply pure_wp_bind, pure_wp_mono_ret; eauto.
 Qed.
+
+Lemma pure_wp_try_compat {A' A E E' φ ψ φ' ψ'} m (f : A → micro A' E') (h : E → micro A' E') :
+  pure_wp m φ ψ →
+  (∀ a, φ a → pure_wp (f a) φ' ψ') →
+  (∀ e, ψ e → pure_wp (h e) φ' ψ') →
+  pure_wp (try m f h) φ' ψ'.
+Proof.
+  intros. eapply pure_wp_try, pure_wp_mono; eauto.
+Qed.
+
+
+(** Versions with [pure_wpv] *)
+
+Lemma pure_wpv_try2_compat {A' A E E' φ φ'} m (f : outcome2 A E → micro A' E') :
+  pure_wpv m φ →
+  (∀ a, φ a → pure_wpv (continue f a) φ') →
+  pure_wpv (try2 m f) φ'.
+Proof.
+  intros; eapply pure_wp_try2_compat; eauto. intros _ [].
+Qed.
+
+Lemma pure_wpv_try2 {A' A E E' φ} m (f : outcome2 A E → micro A' E') :
+  pure_wpv m (λ a, pure_wpv (continue f a) φ) →
+  pure_wpv (try2 m f) φ.
+Proof.
+  intros; eapply pure_wp_try2_compat; eauto. intros _ [].
+Qed.
+
+Lemma pure_wpv_bind {A' A E φ} m (k : A → micro A' E) :
+  pure_wpv m (λ a, pure_wpv (k a) φ) →
+  pure_wpv (bind m k) φ.
+Proof.
+  intros; eapply pure_wp_bind_compat; eauto.
+Qed.
+
+Lemma pure_wpv_try {A' A E E' φ} m (f : A → micro A' E') (h : E → micro A' E') :
+  pure_wpv m (λ a, pure_wpv (f a) φ) →
+  pure_wpv (try m f h) φ.
+Proof.
+  intros; eapply pure_wp_try2_compat; eauto. intros _ [].
+Qed.
+
+Lemma pure_wpv_orelse {A E} (m1 m2 : micro A E) φ :
+  pure_wpv m1 φ →
+  pure_wpv (orelse m1 m2) φ.
+Proof.
+  intros; eapply pure_wp_orelse; eauto. intros _ [].
+Qed.
+
+Lemma pure_wpv_bind_compat {A' A E} (φ : A → Prop) (φ' : A' → Prop) (m : micro A E) k :
+  pure_wpv m φ →
+  (∀ a, φ a → pure_wpv (k a) φ') →
+  pure_wpv (bind m k) φ'.
+Proof.
+  intros; eapply pure_wp_bind_compat; eauto.
+Qed.
+
+Lemma pure_wpv_try_compat {A' A E E' φ φ'} m (f : A → micro A' E') (h : E → micro A' E') :
+  pure_wpv m φ →
+  (∀ a, φ a → pure_wpv (f a) φ') →
+  pure_wpv (try m f h) φ'.
+Proof.
+  intros; eapply pure_wp_try_compat; eauto. intros _ [].
+Qed.
+
 
 
 (** Characterization of [pure_wp] : a computation [m] satisfies some [pure_wp]
@@ -652,6 +728,16 @@ Proof.
     + destruct M as (e1 & -> & ->). apply Hthr. left. eapply invert_pure_wp_throw; eauto.
     + destruct M as (e2 & -> & ->). apply Hthr. right. eapply invert_pure_wp_throw; eauto.
     + destruct M as [[-> | ->] _]; exfalso; eapply invert_pure_wp_crash; eauto.
+Qed.
+
+(* TODO many lemma should be called [Par], not [par] *)
+Lemma pure_wp__par {A1 A2 E} (m1 m2 : micro _ E) φ1 φ2 (φ : A1 * A2 → Prop) ψ :
+  pure_wp m1 φ1 ψ →
+  pure_wp m2 φ2 ψ →
+  (∀ a1 a2, φ1 a1 → φ2 a2 → φ (a1, a2)) →
+  pure_wp (par m1 m2) φ ψ.
+Proof.
+  intros; eapply pure_wp_par_compat; firstorder eauto using pure_wp_ret, pure_wp_throw.
 Qed.
 
 (* simpler version disallowing exceptions *)
